src/program_proof/mvcc/wrbuf_proof.v
@@ -1,0 +1,661 @@
+(* Import definitions/theorems of the Perennial framework with the disk FFI. *)
+From Perennial.program_proof Require Export grove_prelude.
+(* Import Coq model of our Goose program. *)
+From Goose.github_com.mit_pdos.go_mvcc Require Import wrbuf.
+(* Need this for [dbval] and [dbmap], maybe move them out to a separate file? *)
+From Perennial.program_proof.mvcc Require Import mvcc_ghost mvcc_misc.
+(* prefer untyped slices *)
+Import Perennial.goose_lang.lib.slice.slice.
+
+Section heap.
+Context `{!heapGS Σ, !mvcc_ghostG Σ}.
+
+Definition wrent := (u64 * u64 * bool)%type.
+
+Definition wrent_to_val (x : wrent) :=
+  (#x.1.1, (#x.1.2, (#x.2, #())))%V.
+
+Local Definition to_dbval (d : bool) (v : u64) :=
+  if d then Nil else Value v.
+
+Local Definition wrent_to_key_dbval (x : wrent) : (u64 * dbval) :=
+  (x.1.1, (to_dbval x.2 x.1.2)).
+
+Definition own_wrbuf (wrbuf : loc) (mods : dbmap) : iProp Σ :=
+  ∃ (entsS : Slice.t) (ents : list wrent),
+    "Hents"   ∷ wrbuf ↦[WrBuf :: "ents"] (to_val entsS) ∗
+    "HentsS"  ∷ slice.is_slice entsS (structTy WrEnt) 1 (wrent_to_val <$> ents) ∗
+    "%HNoDup" ∷ ⌜NoDup ents.*1.*1⌝ ∗
+    "%Hmods"  ∷ ⌜mods = (list_to_map (wrent_to_key_dbval <$> ents))⌝.
+Hint Extern 1 (environments.envs_entails _ (own_wrbuf _ _)) => unfold own_wrbuf : core.
+
+Local Lemma val_to_wrent_with_val_ty (x : val) :
+  val_ty x (uint64T * (uint64T * (boolT * unitT))%ht) ->
+  (∃ (k : u64) (v : u64) (d : bool), x = wrent_to_val (k, v, d)).
+Proof.
+  intros H.
+  inversion_clear H. 
+  { inversion H0. }
+  inversion_clear H0.
+  inversion_clear H.
+  inversion_clear H1.
+  { inversion H. }
+  inversion_clear H.
+  inversion_clear H1.
+  inversion_clear H0.
+  { inversion H. }
+  inversion_clear H.
+  inversion_clear H0.
+  inversion_clear H1.
+  inversion_clear H.
+  exists x0, x1, x2.
+  unfold wrent_to_val.
+  reflexivity.
+Qed.
+
+Definition spec_search (key : u64) (ents : list wrent) (pos : u64) (found : bool) :=
+  match found with
+  | false => key ∉ ents.*1.*1
+  | true  => (∃ ent, ents !! (int.nat pos) = Some ent ∧ ent.1.1 = key)
+  end.
+
+(*****************************************************************)
+(* func search(ents []WrEnt, key uint64) (uint64, bool)          *)
+(*****************************************************************)
+Local Lemma wp_search (key : u64) (entsS : Slice.t) (ents : list wrent) :
+  {{{ slice.is_slice entsS (structTy WrEnt) 1 (wrent_to_val <$> ents) }}}
+    search (to_val entsS) #key
+  {{{ (pos : u64) (found : bool), RET (#pos, #found);
+      slice.is_slice entsS (structTy WrEnt) 1 (wrent_to_val <$> ents) ∗
+      ⌜spec_search key ents pos found⌝
+  }}}.
+Proof.
+  iIntros (Φ) "HentsS HΦ".
+  wp_call.
+  
+  (***********************************************************)
+  (* var pos uint64 = 0                                      *)
+  (***********************************************************)
+  wp_apply (wp_ref_to); first auto.
+  iIntros (posR) "HposR".
+  wp_pures.
+  
+  (***********************************************************)
+  (* for {                                                   *)
+  (*     if pos >= uint64(len(ents)) {                       *)
+  (*         break                                           *)
+  (*     }                                                   *)
+  (*     if key == ents[pos].key {                           *)
+  (*         break                                           *)
+  (*     }                                                   *)
+  (*     pos++                                               *)
+  (* }                                                       *)
+  (***********************************************************)
+  set P := (λ (b : bool), ∃ (pos : u64),
+               "HentsS" ∷ (slice.is_slice entsS (struct.t WrEnt) 1 (wrent_to_val <$> ents)) ∗
+               "HposR" ∷ posR ↦[uint64T] #pos ∗
+               "%Hpos" ∷ (⌜(int.Z pos) ≤ (int.Z entsS.(Slice.sz))⌝) ∗
+               "%Hexit" ∷ (⌜if b then True
+                            else (∃ (ent : wrent), ents !! (int.nat pos) = Some ent ∧ ent.1.1 = key) ∨
+                                 (int.Z entsS.(Slice.sz)) ≤ (int.Z pos)⌝) ∗
+               "%Hnotin" ∷ (⌜key ∉ (take (int.nat pos) ents.*1.*1)⌝))%I.
+  wp_apply (wp_forBreak P with "[] [$HentsS HposR]").
+  { clear Φ.
+    iIntros (Φ) "!> HP HΦ".
+    iNamed "HP".
+    wp_pures.
+    wp_apply (wp_slice_len).
+    wp_load.
+    wp_if_destruct.
+    { iApply "HΦ". unfold P. eauto 10 with iFrame. }
+    wp_load.
+    iDestruct (slice.is_slice_small_acc with "HentsS") as "[HentsS HentsC]".
+    iDestruct (slice.is_slice_small_sz with "[$HentsS]") as "%HentsSz".
+    destruct (list_lookup_lt _ (wrent_to_val <$> ents) (int.nat pos)) as [ent HSome].
+    { apply Z.nle_gt in Heqb.
+      word.
+    }
+    wp_apply (slice.wp_SliceGet with "[HentsS]"); first auto.
+    iIntros "[HentsS %HentsT]".
+    iDestruct ("HentsC" with "HentsS") as "HentsS".
+    destruct (val_to_wrent_with_val_ty _ HentsT) as (k & v & d & Hent).
+    subst ent.
+    wp_pures.
+    wp_if_destruct.
+    { iApply "HΦ".
+      iModIntro.
+      unfold P.
+      iExists pos.
+      iFrame.
+      iPureIntro.
+      split; first done.
+      split; last done.
+      left.
+      exists (k, v, d).
+      split; last done.
+      rewrite list_lookup_fmap in HSome.
+      apply fmap_Some in HSome as [ent [HSome H]].
+      rewrite HSome.
+      f_equal.
+      inversion H.
+      by rewrite -(surjective_pairing ent.1) -(surjective_pairing ent).
+    }
+    wp_load.
+    wp_pures.
+    wp_store.
+    iModIntro.
+    iApply "HΦ".
+    iFrame.
+    iExists (word.add pos 1%Z).
+    iFrame.
+    iPureIntro.
+    split; first word.
+    split; first done.
+    replace (int.nat (word.add pos 1)) with (S (int.nat pos)); last word.
+    apply Z.nle_gt in Heqb.
+    rewrite (take_S_r _ _ k); last first.
+    { rewrite list_lookup_fmap in HSome.
+      apply fmap_Some in HSome as [ent [HSome H]].
+      inversion H.
+      do 2 rewrite list_lookup_fmap.
+      rewrite HSome.
+      done.
+    }
+    apply not_elem_of_app.
+    split; first done.
+    simpl.
+    rewrite elem_of_list_singleton.
+    unfold not.
+    intros Eqkey.
+    rewrite Eqkey in Heqb0.
+    contradiction.
+  }
+  { iExists (U64 0).
+    iFrame.
+    iPureIntro.
+    change (int.nat 0) with 0%nat.
+    rewrite take_0.
+    split; first word.
+    split; auto using not_elem_of_nil.
+  }
+  iIntros "HP".
+  iNamed "HP".
+  wp_pures.
+  
+  (***********************************************************)
+  (* found := pos < uint64(len(wset))                        *)
+  (* return pos, found                                       *)
+  (***********************************************************)
+  wp_load.
+  wp_apply (wp_slice_len).
+  wp_pures.
+  wp_load.
+  iDestruct (is_slice_sz with "HentsS") as "%Hsz".
+  rewrite fmap_length in Hsz.
+  case_bool_decide; (wp_pures; iModIntro; iApply "HΦ"; iFrame; iPureIntro; unfold spec_search).
+  { (* Write entry found. *)
+    destruct Hexit; [done | word].
+  }
+  { (* Write entry not found. *)
+    apply Z.nlt_ge in H.
+    rewrite take_ge in Hnotin; first done.
+    do 2 rewrite fmap_length.
+    rewrite Hsz.
+    word.
+  }
+Qed.
+
+(* TODO: add meaningful pre/post *)
+Theorem wp_wrent__Key (ent : wrent) :
+  {{{ True }}}
+    WrEnt__Key (wrent_to_val ent)
+  {{{ (key : u64), RET #key; True }}}.
+Proof.
+  iIntros (Φ) "HP HΦ".
+  wp_call.
+  by iApply "HΦ".
+Qed.
+
+Local Lemma NoDup_wrent_to_key_dbval (ents : list wrent) :
+  NoDup ents.*1.*1 ->
+  NoDup (wrent_to_key_dbval <$> ents).*1.
+Proof.
+  intros H.
+  replace (wrent_to_key_dbval <$> _).*1 with ents.*1.*1; last first.
+  { do 2 rewrite -list_fmap_compose. f_equal. }
+  done.
+Qed.
+
+Local Lemma wrent_to_key_dbval_key_fmap (ents : list wrent) :
+  (wrent_to_key_dbval <$> ents).*1 = ents.*1.*1.
+Proof.
+  do 2 rewrite -list_fmap_compose.
+  by apply list_fmap_ext; last done.
+Qed.
+
+Local Lemma NoDup_app_commute (A : Type) (l1 l2 : list A) :
+  NoDup (l1 ++ l2) -> NoDup (l2 ++ l1).
+Proof.
+  intros H.
+  apply NoDup_app in H as (H1 & H2 & H3).
+  apply NoDup_app.
+  split; first done.
+  split; last done.
+  intros x Hl2 Hl1.
+  apply H2 in Hl1.
+  contradiction.
+Qed.
+
+(* TODO: Return values first or others first? Make it consistent. *)
+Definition spec_wrbuf__Lookup (v : u64) (d ok : bool) (key : u64) (m : gmap u64 dbval) :=
+  if ok then m !! key = Some (to_dbval d v) else m !! key = None.
+
+(*****************************************************************)
+(* func (wrbuf *WrBuf) Lookup(key uint64) (uint64, bool, bool)   *)
+(*****************************************************************)
+Theorem wp_wrbuf__Lookup wrbuf (key : u64) m :
+  {{{ own_wrbuf wrbuf m }}}
+    WrBuf__Lookup #wrbuf #key
+  {{{ (v : u64) (d ok : bool), RET (#v, #d, #ok);
+      own_wrbuf wrbuf m ∗ ⌜spec_wrbuf__Lookup v d ok key m⌝
+  }}}.
+Proof.
+  iIntros (Φ) "Hwrbuf HΦ".
+  wp_call.
+  iNamed "Hwrbuf".
+  
+  (***********************************************************)
+  (* pos, found := search(wrbuf.ents, key)                   *)
+  (***********************************************************)
+  wp_loadField.
+  wp_apply (wp_search with "HentsS").
+  iIntros (pos found) "[HentsS %Hsearch]".
+  wp_pures.
+  
+  (***********************************************************)
+  (* if found {                                              *)
+  (*     ent := wrbuf.ents[pos]                              *)
+  (*     return ent.val, ent.del, true                       *)
+  (* }                                                       *)
+  (* return 0, false, false                                  *)
+  (***********************************************************)
+  iDestruct (is_slice_small_acc with "HentsS") as "[HentsS HentsC]".
+  wp_if_destruct.
+  { (* cache hit *)
+    wp_loadField.
+    unfold spec_search in Hsearch.
+    destruct Hsearch as (ent & Hlookup & Hkey).
+    wp_apply (wp_SliceGet with "[HentsS]").
+    { iFrame.
+      iPureIntro.
+      by rewrite list_lookup_fmap Hlookup.
+    }
+    iIntros "[HentsS %Hty]".
+    iDestruct ("HentsC" with "HentsS") as "HentsS".
+    wp_pures.
+    iApply "HΦ".
+    iModIntro.
+    iSplit; first eauto with iFrame.
+    iPureIntro.
+    unfold spec_wrbuf__Lookup.
+    rewrite Hmods.
+    rewrite -elem_of_list_to_map; last by apply NoDup_wrent_to_key_dbval.
+    apply elem_of_list_fmap_1_alt with ent.
+    { by apply elem_of_list_lookup_2 with (int.nat pos). }
+    { rewrite -Hkey. auto using surjective_pairing. }
+  }
+  (* cache miss *)
+  iDestruct ("HentsC" with "HentsS") as "HentsS".
+  wp_pures.
+  iApply "HΦ".
+  iModIntro.
+  iSplit; first eauto with iFrame.
+  iPureIntro.
+  unfold spec_search in Hsearch.
+  unfold spec_wrbuf__Lookup.
+  rewrite Hmods.
+  apply not_elem_of_list_to_map.
+  by rewrite wrent_to_key_dbval_key_fmap.
+Qed.
+
+
+(*****************************************************************)
+(* func (wrbuf *WrBuf) Put(key, val uint64)                      *)
+(*****************************************************************)
+Theorem wp_wrbuf__Put wrbuf (key : u64) (val : u64) m :
+  {{{ own_wrbuf wrbuf m }}}
+    WrBuf__Put #wrbuf #key #val
+  {{{ RET #(); own_wrbuf wrbuf (<[ key := Value val ]> m) }}}.
+Proof.
+  iIntros (Φ) "Hwrbuf HΦ".
+  wp_call.
+  iNamed "Hwrbuf".
+
+  (***********************************************************)
+  (* pos, found := search(wrbuf.ents, key)                   *)
+  (***********************************************************)
+  wp_loadField.
+  wp_apply (wp_search with "HentsS").
+  iIntros (pos found) "[HentsS %Hsearch]".
+  wp_pures.
+
+  (***********************************************************)
+  (* if found {                                              *)
+  (*     ent := &wrbuf.ents[pos]                             *)
+  (*     ent.val = val                                       *)
+  (*     ent.del = false                                     *)
+  (*     return                                              *)
+  (* }                                                       *)
+  (***********************************************************)
+  iDestruct (is_slice_small_acc with "HentsS") as "[HentsS HentsC]".
+  wp_if_destruct.
+  { (* cache hit *)
+    wp_loadField.
+    (* Handling [SliceRef]; a spec would help. *)
+    wp_lam.
+    wp_pures.
+    unfold spec_search in Hsearch.
+    destruct Hsearch as (ent & Hlookup & Hkey).
+    wp_apply (wp_slice_len).
+    iDestruct (is_slice_small_sz with "HentsS") as "%HentsSz".
+    rewrite fmap_length in HentsSz.
+    wp_if_destruct; first last.
+    { destruct Heqb0.
+      apply lookup_lt_Some in Hlookup.
+      rewrite HentsSz in Hlookup. word.
+    }
+    wp_apply (wp_slice_ptr).
+    wp_pures.
+    unfold is_slice_small.
+    iDestruct "HentsS" as "[HentsA [%HentsLen %HentsCap]]".
+    iDestruct (update_array (off:=int.nat pos) with "HentsA") as "[HentsP HentsA]".
+    { by rewrite list_lookup_fmap Hlookup. }
+    iDestruct (struct_fields_split with "HentsP") as "HentsP".
+    iNamed "HentsP".
+    (* update [val] *)
+    wp_apply (wp_storeField with "[val]"); first auto.
+    { iNext.
+      iExactEq "val".
+      do 3 f_equal.
+      word.
+    }
+    iIntros "val".
+    wp_pures.
+    (* update [del] *)
+    wp_apply (wp_storeField with "[del]"); first auto.
+    { iNext.
+      iExactEq "del".
+      do 3 f_equal.
+      word.
+    }
+    iIntros "del".
+    word_cleanup.
+    set entR := (entsS.(Slice.ptr) +ₗ[_] (int.Z pos)).
+    set ent' := (ent.1.1, val, false).
+    iDestruct (struct_fields_split entR 1%Qp WrEnt (wrent_to_val ent')
+                with "[key val del]") as "HentsP".
+    { rewrite /struct_fields. by iFrame. }
+    iDestruct ("HentsA" with "HentsP") as "HentsA".
+    iDestruct ("HentsC" with "[HentsA]") as "HentsS".
+    { iFrame.
+      iPureIntro.
+      by rewrite -HentsLen insert_length.
+    }
+    wp_pures.
+    iApply "HΦ".
+    iModIntro.
+    unfold own_wrbuf.
+    do 2 iExists _.
+    iFrame.
+    iSplit; first by rewrite -list_fmap_insert.
+    iPureIntro.
+    split.
+    { (* prove [NoDup] *)
+      do 2 rewrite list_fmap_insert.
+      subst ent'.
+      simpl.
+      replace (<[ _ := _ ]> ents.*1.*1) with ents.*1.*1; first done.
+      symmetry.
+      apply list_insert_id.
+      do 2 rewrite list_lookup_fmap.
+      by rewrite Hlookup.
+    }
+    { (* prove insertion to list -> insertion to map representation *)
+      rewrite Hmods.
+      rewrite list_fmap_insert.
+      subst ent' key. unfold wrent_to_key_dbval. simpl.
+      apply list_to_map_insert with (to_dbval ent.2 ent.1.2); first by apply NoDup_wrent_to_key_dbval.
+      by rewrite list_lookup_fmap Hlookup.
+    }
+  }
+    
+  (***********************************************************)
+  (* ent := WrEnt {                                          *)
+  (*     key : key,                                          *)
+  (*     val : val,                                          *)
+  (*     del : false,                                        *)
+  (* }                                                       *)
+  (* wrbuf.ents = append(wrbuf.ents, ent)                    *)
+  (***********************************************************)
+  wp_pures.
+  wp_loadField.
+  iDestruct ("HentsC" with "HentsS") as "HentsS".
+  wp_apply (wp_SliceAppend' with "[HentsS]"); [auto 10 | auto 10 | iFrame |].
+  iIntros (entsS') "HentsS".
+  wp_storeField.
+  
+  (* return, cache hit *)
+  iModIntro.
+  iApply "HΦ".
+  unfold spec_search in Hsearch.
+  set ents' := (ents ++ [(key, val, false)]).
+  unfold own_wrbuf.
+
+  iExists _, ents'.
+  iFrame.
+  iSplit; first by rewrite fmap_app.
+  iPureIntro.
+  split.
+  { (* prove [NoDup] *)
+    do 2 rewrite fmap_app.
+    simpl.
+    apply NoDup_app_commute.
+    apply NoDup_app.
+    split; first by apply NoDup_singleton.
+    split; last done.
+    intros x H.
+    apply elem_of_list_singleton in H.
+    by subst x.
+  }
+  { (* prove insertion to list -> insertion to map representation *)
+    symmetry.
+    rewrite Hmods.
+    subst ents'.
+    rewrite fmap_app.
+    apply list_to_map_snoc.
+    by rewrite wrent_to_key_dbval_key_fmap.
+  }
+Qed.
+
+(*****************************************************************)
+(* func (wrbuf *WrBuf) Delete(key uint64)                        *)
+(*****************************************************************)
+Theorem wp_wrbuf__Delete wrbuf (key : u64) m :
+  {{{ own_wrbuf wrbuf m }}}
+    WrBuf__Delete #wrbuf #key
+  {{{ RET #(); own_wrbuf wrbuf (<[ key := Nil ]> m) }}}.
+Proof.
+  iIntros (Φ) "Hwrbuf HΦ".
+  wp_call.
+  iNamed "Hwrbuf".
+
+  (***********************************************************)
+  (* pos, found := search(wrbuf.ents, key)                   *)
+  (***********************************************************)
+  wp_loadField.
+  wp_apply (wp_search with "HentsS").
+  iIntros (pos found) "[HentsS %Hsearch]".
+  wp_pures.
+
+  (***********************************************************)
+  (* if found {                                              *)
+  (*     ent := &wrbuf.ents[pos]                             *)
+  (*     ent.del = true                                      *)
+  (*     return                                              *)
+  (* }                                                       *)
+  (***********************************************************)
+  iDestruct (is_slice_small_acc with "HentsS") as "[HentsS HentsC]".
+  wp_if_destruct.
+  { (* cache hit *)
+    wp_loadField.
+    (* Handling [SliceRef]; a spec would help. *)
+    wp_lam.
+    wp_pures.
+    unfold spec_search in Hsearch.
+    destruct Hsearch as (ent & Hlookup & Hkey).
+    wp_apply (wp_slice_len).
+    iDestruct (is_slice_small_sz with "HentsS") as "%HentsSz".
+    rewrite fmap_length in HentsSz.
+    wp_if_destruct; first last.
+    { destruct Heqb0.
+      apply lookup_lt_Some in Hlookup.
+      rewrite HentsSz in Hlookup. word.
+    }
+    wp_apply (wp_slice_ptr).
+    wp_pures.
+    unfold is_slice_small.
+    iDestruct "HentsS" as "[HentsA [%HentsLen %HentsCap]]".
+    iDestruct (update_array (off:=int.nat pos) with "HentsA") as "[HentsP HentsA]".
+    { by rewrite list_lookup_fmap Hlookup. }
+    iDestruct (struct_fields_split with "HentsP") as "HentsP".
+    iNamed "HentsP".
+    (* update [del] *)
+    wp_apply (wp_storeField with "[del]"); first auto.
+    { iNext.
+      iExactEq "del".
+      do 3 f_equal.
+      word.
+    }
+    iIntros "del".
+    word_cleanup.
+    set entR := (entsS.(Slice.ptr) +ₗ[_] (int.Z pos)).
+    set ent' := (ent.1.1, ent.1.2, true).
+    iDestruct (struct_fields_split entR 1%Qp WrEnt (wrent_to_val ent')
+                with "[key val del]") as "HentsP".
+    { rewrite /struct_fields. by iFrame. }
+    iDestruct ("HentsA" with "HentsP") as "HentsA".
+    iDestruct ("HentsC" with "[HentsA]") as "HentsS".
+    { iFrame.
+      iPureIntro.
+      by rewrite -HentsLen insert_length.
+    }
+    wp_pures.
+    iApply "HΦ".
+    iModIntro.
+    unfold own_wrbuf.
+    do 2 iExists _.
+    iFrame.
+    iSplit; first by rewrite -list_fmap_insert.
+    iPureIntro.
+    split.
+    { (* prove [NoDup] *)
+      do 2 rewrite list_fmap_insert.
+      subst ent'.
+      simpl.
+      replace (<[ _ := _ ]> ents.*1.*1) with ents.*1.*1; first done.
+      symmetry.
+      apply list_insert_id.
+      do 2 rewrite list_lookup_fmap.
+      by rewrite Hlookup.
+    }
+    { (* prove insertion to list -> insertion to map representation *)
+      rewrite Hmods.
+      rewrite list_fmap_insert.
+      subst ent' key. unfold wrent_to_key_dbval. simpl.
+      apply list_to_map_insert with (to_dbval ent.2 ent.1.2); first by apply NoDup_wrent_to_key_dbval.
+      by rewrite list_lookup_fmap Hlookup.
+    }
+  }
+    
+  (***********************************************************)
+  (* ent := WrEnt {                                          *)
+  (*     key : key,                                          *)
+  (*     del : true,                                         *)
+  (* }                                                       *)
+  (* wrbuf.ents = append(wrbuf.ents, ent)                    *)
+  (***********************************************************)
+  wp_pures.
+  wp_loadField.
+  iDestruct ("HentsC" with "HentsS") as "HentsS".
+  wp_apply (wp_SliceAppend' with "[HentsS]"); [auto 10 | auto 10 | iFrame |].
+  iIntros (entsS') "HentsS".
+  wp_storeField.
+  
+  (* return, cache hit *)
+  iModIntro.
+  iApply "HΦ".
+  unfold spec_search in Hsearch.
+  (* [(U64 0)] is the zero-value of [u64]. *)
+  set ents' := (ents ++ [(key, (U64 0), true)]).
+  unfold own_wrbuf.
+
+  iExists _, ents'.
+  iFrame.
+  iSplit; first by rewrite fmap_app.
+  iPureIntro.
+  split.
+  { (* prove [NoDup] *)
+    do 2 rewrite fmap_app.
+    simpl.
+    apply NoDup_app_commute.
+    apply NoDup_app.
+    split; first by apply NoDup_singleton.
+    split; last done.
+    intros x H.
+    apply elem_of_list_singleton in H.
+    by subst x.
+  }
+  { (* prove insertion to list -> insertion to map representation *)
+    symmetry.
+    rewrite Hmods.
+    subst ents'.
+    rewrite fmap_app.
+    apply list_to_map_snoc.
+    by rewrite wrent_to_key_dbval_key_fmap.
+  }
+Qed.
+
+(*****************************************************************)
+(* (wrbuf *WrBuf) Clear()                                        *)
+(*****************************************************************)
+Theorem wp_wrbuf__Clear wrbuf m :
+  {{{ own_wrbuf wrbuf m }}}
+    WrBuf__Clear #wrbuf
+  {{{ RET #(); own_wrbuf wrbuf ∅ }}}.
+Proof.
+  iIntros (Φ) "Hwrbuf HΦ".
+  wp_call.
+  iNamed "Hwrbuf".
+
+  (***********************************************************)
+  (* wrbuf.ents = wrbuf.ents[ : 0]                           *)
+  (***********************************************************)
+  wp_loadField.
+  wp_apply (wp_SliceTake); first word.
+  wp_apply (wp_storeField with "Hents"); first eauto.
+  iIntros "Hents".
+  wp_pures.
+
+  iApply "HΦ".
+  iModIntro.
+  iExists _, [].
+  iDestruct (is_slice_take_cap _ _ _ (U64 0) with "HentsS") as "HentsS"; first word.
+  change (int.nat 0) with 0%nat.
+  rewrite take_0.
+  do 2 rewrite fmap_nil.
+  iFrame.
+  iPureIntro.
+  split; [apply NoDup_nil_2 | done].
+Qed.
+
+End heap.
